unused.v
@@ -17,3 +17,41 @@ Proof.
   elim (in_empty Hy).
 Qed.
 
+Lemma subset_remove_both : forall v L1 L2,
+  L1 << L2 -> S.remove v L1 << S.remove v L2.
+Proof.
+  intros.
+  intros y Hy.
+  destruct (v == y).
+    elim (S.remove_1 e Hy).
+  apply* S.remove_2.
+  apply H.
+  apply* S.remove_3.
+Qed.
+
+Lemma binds_subst_dom : forall (A:Set) x (a:A) Xs Ys Ks L,
+  fresh L (length Xs) Ys ->
+  binds x a (combine Xs Ks) ->
+  exists y,
+    binds x (typ_fvar y) (combine Xs (typ_fvars Ys)) /\
+    binds y a (combine Ys Ks).
+Proof.
+  induction Xs; destruct Ys; intros; try discriminate.
+    contradiction.
+  destruct Ks. discriminate.
+  unfold binds in *; simpl in *.
+  destruct (x == a0).
+    esplit; split*. destruct* (v == v).
+  destruct* (IHXs Ys Ks (L \u {{v}})) as [y [Bx By]].
+  esplit; split*.
+  destruct* (y == v).
+  subst.
+  destruct (fresh_disjoint _ _ _ (proj2 H) v).
+    elim H1.
+    use (binds_combine _ _ Bx).
+    unfold typ_fvars in H2.
+    destruct (proj1 (in_map_iff _ _ _) H2).
+    destruct H3. inversions H3.
+    apply* in_mkset.
+  notin_contradiction.
+Qed.
